Rewrite of label-free (logic) language - labels as part of syntax

label-free/Syntax.v
@@ -1,3 +1,5 @@
+Require Import Metatheory.
+
 Inductive ty_LF :=
 | tvar_LF: ty_LF
 | tarrow_LF: ty_LF -> ty_LF -> ty_LF
@@ -11,7 +13,13 @@ Notation " '<*>' A " := (tdia_LF A) (at level 30) : label_free_is5_scope.
 
 Open Scope label_free_is5_scope.
 
-Definition Context_LF := list ty_LF.
+Definition Context_LF := prod var (list ty_LF).
+Definition Background_LF := list Context_LF.
+
+Inductive ctx_LF :=
+| bctx: nat -> ctx_LF
+| fctx: var -> ctx_LF.
+
 
 Inductive te_LF :=
 | hyp_LF: nat -> te_LF
@@ -19,12 +27,32 @@ Inductive te_LF :=
 | appl_LF: te_LF -> te_LF -> te_LF
 | box_LF: te_LF -> te_LF
 | unbox_LF: te_LF -> te_LF
-| unbox_fetch_LF: te_LF -> Context_LF -> te_LF
+| unbox_fetch_LF: ctx_LF -> te_LF -> te_LF
 | here_LF: te_LF -> te_LF
-| get_here_LF: te_LF -> Context_LF -> te_LF
+| get_here_LF: ctx_LF -> te_LF -> te_LF
 | letdia_LF: te_LF -> te_LF -> te_LF
-| letdia_get_LF: te_LF -> te_LF -> Context_LF -> te_LF
+| letdia_get_LF: ctx_LF -> te_LF -> te_LF -> te_LF
 .
+
+Axiom eq_var_LF_dec:
+  forall v1 v2: var, {v1 = v2} + {v1 <> v2}.
+
+Theorem eq_context_LF_dec:
+forall c1 c2: Context_LF, {c1 = c2} + {c1 <> c2}.
+intros.
+decide equality.
+decide equality.
+decide equality.
+apply eq_var_LF_dec.
+Qed.
+
+Theorem eq_ctx_LF_dec:
+forall c1 c2: ctx_LF, {c1 = c2} + {c1 <> c2}.
+intros.
+decide equality.
+decide equality.
+apply eq_var_LF_dec. 
+Qed.
 
 Theorem eq_ty_LF_dec:
 forall t1 t2: ty_LF, {t1 = t2} + {t1 <> t2}.
@@ -36,16 +64,9 @@ forall t1 t2: te_LF, {t1 = t2} + {t1 <> t2}.
 intros; decide equality.
 decide equality.
 decide equality.
-decide equality; decide equality.
-decide equality; decide equality.
-decide equality; decide equality.
-Qed.
-
-Theorem eq_context_LF_dec:
-forall c1 c2: Context_LF, {c1 = c2} + {c1 <> c2}.
-intros.
-decide equality.
-decide equality.
+apply eq_ctx_LF_dec.
+apply eq_ctx_LF_dec.
+apply eq_ctx_LF_dec.
 Qed.
 
 Close Scope label_free_is5_scope.
